soundness/FallingEdge.v
@@ -15,12 +15,12 @@ Require Import hvhdl.HilecopDesignStore.
 
 Require Import sitpn2hvhdl.GenerateHVhdl.
 
-Require Import soundness.SoundnessDefs.
+Require Import soundness.SemanticPreservationDefs.
 
 (** ** Falling Edge Lemma *)
 
-Lemma falling_edge :
-  forall sitpn decpr id__ent id__arch mm d γ E__c E__p Δ σ__e s σ τ s' σ__injf σ__f σ',
+Lemma falling_edge_full :
+  forall sitpn decpr id__ent id__arch mm d γ E__c E__p Δ σ__e s σ τ s' σ__f σ',
 
     (* sitpn translates into (d, γ). *)
     sitpn_to_hvhdl sitpn decpr id__ent id__arch mm = (inl (d, γ)) ->
@@ -32,18 +32,45 @@ Lemma falling_edge :
     edesign hdstore (empty value) d Δ σ__e ->
 
     (* States s and σ are similar (post rising edge). *)
-    SimStateAfterRE sitpn γ s σ ->
+    @FullSimStateAfterRE sitpn γ E__c τ s σ ->
 
     (* From s to s' after ↓. *)
     SitpnStateTransition E__c τ s s' fe ->
 
     (* From σ to σ' after ↓. *)
-    IsInjectedDState σ (E__p τ fe) σ__injf ->
-    vfalling hdstore Δ σ__injf (behavior d) σ__f ->
+    vfalling hdstore Δ σ (behavior d) σ__f ->
+    stabilize hdstore Δ σ__f (behavior d) σ' ->
+
+    (* States s' and σ' are similar (post falling edge). *)
+    FullSimStateAfterFE sitpn γ s' σ'.
+Admitted.
+
+Hint Resolve falling_edge_full : hilecop.
+
+Lemma falling_edge :
+  forall sitpn decpr id__ent id__arch mm d γ E__c E__p Δ σ__e s σ τ s' σ__f σ',
+
+    (* sitpn translates into (d, γ). *)
+    sitpn_to_hvhdl sitpn decpr id__ent id__arch mm = (inl (d, γ)) ->
+
+    (* Environments are similar. *)
+    SimEnv sitpn γ E__c E__p ->
+    
+    (* [Δ, σ__e] are the results of the elaboration of [d]. *)
+    edesign hdstore (empty value) d Δ σ__e ->
+
+    (* States s and σ are similar (post rising edge). *)
+    @FullSimStateAfterRE sitpn γ E__c τ s σ ->
+
+    (* From s to s' after ↓. *)
+    SitpnStateTransition E__c τ s s' fe ->
+
+    (* From σ to σ' after ↓. *)
+    vfalling hdstore Δ σ (behavior d) σ__f ->
     stabilize hdstore Δ σ__f (behavior d) σ' ->
 
     (* States s' and σ' are similar (post falling edge). *)
     SimStateAfterFE sitpn γ s' σ'.
 Admitted.
 
-Hint Resolve falling_edge : core.
+Hint Resolve falling_edge : hilecop.
