soundness/RisingEdge.v
@@ -15,12 +15,12 @@ Require Import hvhdl.HilecopDesignStore.
 
 Require Import sitpn2hvhdl.GenerateHVhdl.
 
-Require Import soundness.SoundnessDefs.
+Require Import soundness.SemanticPreservationDefs.
 
-(** ** Rising Edge Lemma *)
+(** ** Rising edge lemmas *)
 
-Lemma rising_edge :
-  forall sitpn decpr id__ent id__arch mm d γ E__c E__p Δ σ__e s σ τ s' σ__injr σ__r σ',
+Lemma rising_edge_full :
+  forall sitpn decpr id__ent id__arch mm d γ E__c E__p Δ σ__e s σ τ s' σ__i σ__r σ',
 
     (* sitpn translates into (d, γ). *)
     sitpn_to_hvhdl sitpn decpr id__ent id__arch mm = (inl (d, γ)) ->
@@ -32,18 +32,47 @@ Lemma rising_edge :
     edesign hdstore (empty value) d Δ σ__e ->
 
     (* States s and σ are similar (post falling edge). *)
-    SimStateAfterFE sitpn γ s σ ->
+    FullSimStateAfterFE sitpn γ s σ ->
 
     (* From s to s' after ↑. *)
     SitpnStateTransition E__c τ s s' re ->
 
     (* From σ to σ' after ↑. *)
-    IsInjectedDState σ (E__p τ re) σ__injr ->
-    vrising hdstore Δ σ__injr (behavior d) σ__r ->
+    IsInjectedDState σ (E__p τ) σ__i ->
+    vrising hdstore Δ σ__i (behavior d) σ__r ->
     stabilize hdstore Δ σ__r (behavior d) σ' ->
 
-    (* States s' and σ' are similar (post rising edge). *)
+    (* States s' and σ' are similar (full post rising edge similarity). *)
+    FullSimStateAfterRE sitpn γ E__c τ s' σ'.
+Admitted.
+
+Hint Resolve rising_edge_full : hilecop.
+
+Lemma rising_edge :
+  forall sitpn decpr id__ent id__arch mm d γ E__c E__p Δ σ__e s σ τ s' σ__i σ__r σ',
+
+    (* sitpn translates into (d, γ). *)
+    sitpn_to_hvhdl sitpn decpr id__ent id__arch mm = (inl (d, γ)) ->
+
+    (* Environments are similar. *)
+    SimEnv sitpn γ E__c E__p ->
+    
+    (* [Δ, σ__e] are the results of the elaboration of [d]. *)
+    edesign hdstore (empty value) d Δ σ__e ->
+
+    (* States s and σ are similar (post falling edge). *)
+    FullSimStateAfterFE sitpn γ s σ ->
+
+    (* From s to s' after ↑. *)
+    SitpnStateTransition E__c τ s s' re ->
+
+    (* From σ to σ' after ↑. *)
+    IsInjectedDState σ (E__p τ) σ__i ->
+    vrising hdstore Δ σ__i (behavior d) σ__r ->
+    stabilize hdstore Δ σ__r (behavior d) σ' ->
+
+    (* States s' and σ' are similar (post rising edge similarity). *)
     SimStateAfterRE sitpn γ s' σ'.
 Admitted.
 
-Hint Resolve rising_edge : core.
+Hint Resolve rising_edge : hilecop.
